\section{Равномерное распределение}

\subsection{Определение}
\begin{equation}
	f_\xi(x) = \frac{1}{b-a} \one{[a;b]}(x)
\end{equation}
\subsection{Матожидание}

\begin{multline}
M\xi =  \intl_{-\infty }^{\infty } xf_\xi(x) dx =
\intl_{a }^{b } x \frac{1}{b-a} dx =
\\=
\frac{1}{b-a} \left.  \left( \frac{x^2}{2} \right)   \right|_{ x=a}^{ x=b}=
\frac{b^2-a^2}{2(b-a)}=
\frac{(b-a)(b+a)}{2(b-a)}=
\frac{a+b}{2}
\end{multline}

\subsection{Дисперсия}
\begin{multline}
    M( \xi ^2) = 
    \intl_{-\infty }^{\infty } x^2 \frac{1}{b-a}dx =
    \frac{1}{b-a} \intl_{-\infty }^{\infty } x^2 dx =
    \\=
    \frac{1}{b-a}\left. \left( \frac{x^3}{3} \right)  \right|_{ x=a}^{ x=b} = 
    \frac{1}{b-a} \left( \frac{b^3}{3} - \frac{a^3}{3}\right) =
    \\=
    \frac{1}{b-a} \left( \frac{b^3 - a^3}{3} \right) = 
    \frac{1}{b-a} \left( \frac{(b-a)(a^2+ab+b^2)}{3} \right) = 
    \frac{a^2+ab+b^2}{3}
\end{multline}

\begin{multline}
	D\xi =
	M(\xi^2)-(M\xi)^2 = 
	\frac{a^2+ab+b^2}{3} - \left( \frac{a+b}{2} \right)^2  =
	\\=
	\frac{a^2+ab+b^2}{3} - \frac{a^2+2ab+b^2}{4} =  
	\frac{4a^2+4ab+4b^2}{12} - \frac{3a^2+6ab+3b^2}{12} = 
	\\= 
	\frac{4a^2+4ab+4b^2-3a^2-6ab-3b^2}{12}=  
	\frac{a^2 -2ab + b^2 }{12}=  
	\frac{(a-b)^2}{12}  
\end{multline}

